> Theory and Implementation of Programming Languages
>
> Fall 2020

Hw#3 (30 pts) Grammars (Due Date: Wed Oct. 21, 11:59 PM). Ex#1: Given the following grammar G = (V, T, S, P) where S is the starting symbol.

S → AB

A → Aa

A.  → bB

B.  → a

B → Sb

a\) Is this G regular? yes b) Is G contextffree? yes c) What is the form of G? Chomsky

e)  Give the leftmost and rightmost derivation of baabaab

Leftmost: AB => AaB => bBaB => baaB => baaSb => baaABb => baabBBb => baabaBb => baabaab

Rightmost: AB => ASb => AABb => AAab => AbBab => Abaab => Aabaab => bBabaab => baabaab

f)  Give the parse (derivation) tree of baabaab, bBABb, and baSb

![](media/image1.png){width="1.5208333333333333in" height="2.5104166666666665in"}![](media/image2.png){width="1.15625in" height="1.46875in"}![](media/image3.png){width="0.875in" height="1.5104166666666667in"}

Ex#2: Given the following grammar G = (V, T, S, P) with Float as its starting state for the basic floating=point

numbers.

Float → Integer.Fraction

Integer → Digit \| Integer Digit

Fraction → Digit \| Digit Fraction

Digit → λ \| 0 \| 1 \| 2 \| 3 \| 4 \| 5 \| 6 \| 7 \| 8 \| 9

a)  List the values of V and T

    a.  V = {Float, Integer, Fraction, Digit} T= {0,1,2,3,4,5,6,7,8,9, .}

b)  Give the leftmost derivation of 57.13

> Float => Integer.Fraction => Integer Digit.Fraction => Digit Digit.Fraction => 5 Digit.Fraction => 57.Fraction => 57.Digit Fraction => 57.1 Fraction => 57.1Digit => 57.13Then draw the corresponding parse tree.
>
> ![](media/image4.png){width="2.53125in" height="2.1875in"}

Ex#3: Give a string of lengths, 4, 6, 8 generated by the following grammar G = (V, T, S. P).

S → 0S

S à 0S1S

S à λ

0000, 000000, 00000000

Ex#4: Write the grammar for a Java class definition header statement using Backus-Naur Form (BNF)

Grammar G = (V, T, S, P) where S is the starting symbol

S ::= public class \<string> \| public class \<string> \<choice> \<string>

Choice ::= extends \| implements

String ::= \<firstChar> \<char>

firstChar ::= a....z

Char ::= a...z \| \_ \| 0..9 \| \<char> \<char>

Ex#5: Given the following grammar for a simple assignment statements.

\<assign> à \<id> = \<expr>

\<id> à A \| B \| C

\<exp> à \<id> + \<expr> \| \<id> \* \<expr> \| (\<expr>) \| \<id>

Show a left most derivation and a parse tree of the following statement:

A = A \*(B + (C \* A))

\<assign> => \<id> = \<expr> => A = \<expr> => A = \<id> \* \<expr> => A = A \* \<expr> => A = A \* (\<expr>) => A = A \* (\<id> + \<expr>) => A = A \* (B + \<expr>) => A = A \* (B + (\<expr>)) => A = A \* (B + (\<id> \* \<expr>)) => A = A \* (B + (C \* \<expr>)) => A = A \* (B + (C \* \<id>)) => A = A \* (B + (C \* A))

Ex#6: Prove the following grammar is ambiguous.

\<S> à \<A>

\<A> à \<A> + \<A>

\<A> à \<id>

\<id> à a \| b \| c

S => \<A> => \<A> + \<A> => \<id> + \<A> => \<id> + \<A> => a + \<A> => a + \<A> + \<A> => a + \<id> + \<A> => a + b + \<A> => a + b + \<id> => a + b + b

S => \<A> => \<A> + \<A> => \<A> + \<A> + \<A> => \<id> + \<A> + \<A> => a + \<A> + \<A> => a + \<id> + \<A> => a + b + \<A> => a + b + \<id> => a + b + b
